src/typechecker/FStar.TypeChecker.TcTerm.fs
@@ -3427,30 +3427,21 @@ and build_let_rec_env _top_level env lbs : list<letbinding> * env_t * guard_t =
      //lbdef is of the form (fun x -> t)
      //in which case, we need to add (#'a:Type) to the actuals
      //See the handling in Tm_abs case of tc_value, roughly line 703 (location may have changed since this comment was written)
-     if Env.debug env <| Options.Other "Dec"
-     then BU.print2 "lbtyp=%s, actuals=%s\n" (Print.term_to_string lbtyp) (Print.binders_to_string ", " actuals);
      let actuals = TcUtil.maybe_add_implicit_binders (Env.set_expected_typ env lbtyp) actuals in
      let nactuals = List.length actuals in
-     if Env.debug env <| Options.Other "Dec"
-     then BU.print1 "After add implicit binders actuals=%s\n" (Print.binders_to_string ", " actuals);
 
      (* Grab binders from the type. At most as many as we have in
       * the abstraction. *)
      let formals, c = N.get_n_binders env nactuals lbtyp in
 
-     if Env.debug env <| Options.Other "Dec"
-     then BU.print2 "After get_n_binders: %s -> %s\n" (Print.binders_to_string ", " formals) (Print.comp_to_string c);
-
      // TODO: There's a similar error in check_let_recs, would be nice
      // to remove this one.
      if List.isEmpty formals || List.isEmpty actuals then
        raise_error (Errors.Fatal_RecursiveFunctionLiteral,
-                    (BU.format5 "Only function literals with arrow types can be defined recursively; got (%s) %s : %s; actuals = %s; formals = %s"
+                    (BU.format3 "Only function literals with arrow types can be defined recursively; got (%s) %s : %s"
                                (Print.tag_of_term lbdef)
                                (Print.term_to_string lbdef)
-                               (Print.term_to_string lbtyp)
-                               (Print.binders_to_string ", " actuals)
-                               (Print.binders_to_string ", " formals)))
+                               (Print.term_to_string lbtyp)))
                    lbtyp.pos; // TODO: GM: maybe point to the one that's actually empty?
 
      let nformals = List.length formals in
@@ -3473,12 +3464,6 @@ and build_let_rec_env _top_level env lbs : list<letbinding> * env_t * guard_t =
    in
    let lbs, env, g = List.fold_left (fun (lbs, env, g_acc) lb ->
         let univ_vars, lbtyp, lbdef, check_t = TcUtil.extract_let_rec_annotation env lb in
-        if Env.debug env <| Options.Other "Dec"
-        then BU.print3 "Got lbtyp(should_check=%s)=%s\n\
-                        and lbdef=%s\n"
-                       (BU.string_of_bool check_t)
-                       (Print.term_to_string lbtyp)
-                       (Print.term_to_string lbdef);
         let env = Env.push_univ_vars env univ_vars in //no polymorphic recursion on universes
         let g, lbtyp = 
             if not check_t 
@@ -3519,10 +3504,9 @@ and check_let_recs env lbts =
         //see issue #1017
         match bs with
         | [] -> raise_error (Errors.Fatal_RecursiveFunctionLiteral, 
-                            BU.format3
-                            "Only function literals may be defined recursively; %s is defined to be a %s, i.e., %s"
+                            BU.format2
+                            "Only function literals may be defined recursively; %s is defined to be %s"
                                (Print.lbname_to_string lb.lbname)
-                               (Print.tag_of_term lb.lbdef)
                                (Print.term_to_string lb.lbdef)
                             ) (S.range_of_lbname lb.lbname)
         | _ -> ();
